src/SpecificGen/GF41417_32Reflective/Common10_4Op.v
@@ -1,0 +1,115 @@
+Require Export Crypto.SpecificGen.GF41417_32Reflective.Common.
+Require Import Crypto.SpecificGen.GF41417_32BoundedCommon.
+Require Import Crypto.Reflection.Z.Interpretations64.
+Require Import Crypto.Reflection.Syntax.
+Require Import Crypto.Reflection.Application.
+Require Import Crypto.Reflection.MapInterp.
+Require Import Crypto.Util.Tactics.
+
+Local Opaque Interp.
+Local Notation eta_and x := (let (a, b) := x in a, let (a, b) := x in b) (only parsing).
+Lemma Expr10_4Op_correct_and_bounded
+      ropW op (ropZ_sig : rexpr_10_4op_sig op)
+      (Hbounds : correct_and_bounded_genT ropW ropZ_sig)
+      (H0 : forall x0123456789
+                   (x0123456789
+                    := (eta_fe41417_32W (fst (fst (fst (fst (fst (fst (fst (fst (fst x0123456789))))))))),
+                        eta_fe41417_32W (snd (fst (fst (fst (fst (fst (fst (fst (fst x0123456789))))))))),
+                        eta_fe41417_32W (snd (fst (fst (fst (fst (fst (fst (fst x0123456789)))))))),
+                        eta_fe41417_32W (snd (fst (fst (fst (fst (fst (fst x0123456789))))))),
+                        eta_fe41417_32W (snd (fst (fst (fst (fst (fst x0123456789)))))),
+                        eta_fe41417_32W (snd (fst (fst (fst (fst x0123456789))))),
+                        eta_fe41417_32W (snd (fst (fst (fst x0123456789)))),
+                        eta_fe41417_32W (snd (fst (fst x0123456789))),
+                        eta_fe41417_32W (snd (fst x0123456789)),
+                        eta_fe41417_32W (snd x0123456789)))
+                   (Hx0123456789
+                    : is_bounded (fe41417_32WToZ (fst (fst (fst (fst (fst (fst (fst (fst (fst x0123456789)))))))))) = true
+                      /\ is_bounded (fe41417_32WToZ (snd (fst (fst (fst (fst (fst (fst (fst (fst x0123456789)))))))))) = true
+                      /\ is_bounded (fe41417_32WToZ (snd (fst (fst (fst (fst (fst (fst (fst x0123456789))))))))) = true
+                      /\ is_bounded (fe41417_32WToZ (snd (fst (fst (fst (fst (fst (fst x0123456789)))))))) = true
+                      /\ is_bounded (fe41417_32WToZ (snd (fst (fst (fst (fst (fst x0123456789))))))) = true
+                      /\ is_bounded (fe41417_32WToZ (snd (fst (fst (fst (fst x0123456789)))))) = true
+                      /\ is_bounded (fe41417_32WToZ (snd (fst (fst (fst x0123456789))))) = true
+                      /\ is_bounded (fe41417_32WToZ (snd (fst (fst x0123456789)))) = true
+                      /\ is_bounded (fe41417_32WToZ (snd (fst x0123456789))) = true
+                      /\ is_bounded (fe41417_32WToZ (snd x0123456789)) = true),
+          let (Hx0, Hx123456789) := (eta_and Hx0123456789) in
+          let (Hx1, Hx23456789) := (eta_and Hx123456789) in
+          let (Hx2, Hx3456789) := (eta_and Hx23456789) in
+          let (Hx3, Hx456789) := (eta_and Hx3456789) in
+          let (Hx4, Hx56789) := (eta_and Hx456789) in
+          let (Hx5, Hx6789) := (eta_and Hx56789) in
+          let (Hx6, Hx789) := (eta_and Hx6789) in
+          let (Hx7, Hx89) := (eta_and Hx789) in
+          let (Hx8, Hx9) := (eta_and Hx89) in
+          let args := op10_args_to_bounded x0123456789 Hx0 Hx1 Hx2 Hx3 Hx4 Hx5 Hx6 Hx7 Hx8 Hx9 in
+          match LiftOption.of'
+                  (ApplyInterpedAll (Interp (@BoundedWordW.interp_op) (MapInterp BoundedWordW.of_wordW ropW))
+                                    (LiftOption.to' (Some args)))
+          with
+          | Some _ => True
+          | None => False
+          end)
+      (H1 : forall x0123456789
+                   (x0123456789
+                    := (eta_fe41417_32W (fst (fst (fst (fst (fst (fst (fst (fst (fst x0123456789))))))))),
+                        eta_fe41417_32W (snd (fst (fst (fst (fst (fst (fst (fst (fst x0123456789))))))))),
+                        eta_fe41417_32W (snd (fst (fst (fst (fst (fst (fst (fst x0123456789)))))))),
+                        eta_fe41417_32W (snd (fst (fst (fst (fst (fst (fst x0123456789))))))),
+                        eta_fe41417_32W (snd (fst (fst (fst (fst (fst x0123456789)))))),
+                        eta_fe41417_32W (snd (fst (fst (fst (fst x0123456789))))),
+                        eta_fe41417_32W (snd (fst (fst (fst x0123456789)))),
+                        eta_fe41417_32W (snd (fst (fst x0123456789))),
+                        eta_fe41417_32W (snd (fst x0123456789)),
+                        eta_fe41417_32W (snd x0123456789)))
+                   (Hx0123456789
+                    : is_bounded (fe41417_32WToZ (fst (fst (fst (fst (fst (fst (fst (fst (fst x0123456789)))))))))) = true
+                      /\ is_bounded (fe41417_32WToZ (snd (fst (fst (fst (fst (fst (fst (fst (fst x0123456789)))))))))) = true
+                      /\ is_bounded (fe41417_32WToZ (snd (fst (fst (fst (fst (fst (fst (fst x0123456789))))))))) = true
+                      /\ is_bounded (fe41417_32WToZ (snd (fst (fst (fst (fst (fst (fst x0123456789)))))))) = true
+                      /\ is_bounded (fe41417_32WToZ (snd (fst (fst (fst (fst (fst x0123456789))))))) = true
+                      /\ is_bounded (fe41417_32WToZ (snd (fst (fst (fst (fst x0123456789)))))) = true
+                      /\ is_bounded (fe41417_32WToZ (snd (fst (fst (fst x0123456789))))) = true
+                      /\ is_bounded (fe41417_32WToZ (snd (fst (fst x0123456789)))) = true
+                      /\ is_bounded (fe41417_32WToZ (snd (fst x0123456789))) = true
+                      /\ is_bounded (fe41417_32WToZ (snd x0123456789)) = true),
+          let (Hx0, Hx123456789) := (eta_and Hx0123456789) in
+          let (Hx1, Hx23456789) := (eta_and Hx123456789) in
+          let (Hx2, Hx3456789) := (eta_and Hx23456789) in
+          let (Hx3, Hx456789) := (eta_and Hx3456789) in
+          let (Hx4, Hx56789) := (eta_and Hx456789) in
+          let (Hx5, Hx6789) := (eta_and Hx56789) in
+          let (Hx6, Hx789) := (eta_and Hx6789) in
+          let (Hx7, Hx89) := (eta_and Hx789) in
+          let (Hx8, Hx9) := (eta_and Hx89) in
+          let args := op10_args_to_bounded x0123456789 Hx0 Hx1 Hx2 Hx3 Hx4 Hx5 Hx6 Hx7 Hx8 Hx9 in
+          let x' := SmartVarfMap (fun _ : base_type => BoundedWordW.BoundedWordToBounds) args in
+          match LiftOption.of'
+                  (ApplyInterpedAll (Interp (@ZBounds.interp_op) (MapInterp ZBounds.of_wordW ropW)) (LiftOption.to' (Some x')))
+          with
+          | Some bounds => op10_4_bounds_good bounds = true
+          | None => False
+          end)
+  : op10_4_correct_and_bounded (MapInterp (fun _ x => x) ropW) op.
+Proof.
+  intros x0 x1 x2 x3 x4 x5 x6 x7 x8 x9.
+  intros Hx0 Hx1 Hx2 Hx3 Hx4 Hx5 Hx6 Hx7 Hx8 Hx9.
+  pose x0 as x0'.
+  pose x1 as x1'.
+  pose x2 as x2'.
+  pose x3 as x3'.
+  pose x4 as x4'.
+  pose x5 as x5'.
+  pose x6 as x6'.
+  pose x7 as x7'.
+  pose x8 as x8'.
+  pose x9 as x9'.
+  hnf in x0, x1, x2, x3, x4, x5, x6, x7, x8, x9; destruct_head' prod.
+  specialize (H0 (x0', x1', x2', x3', x4', x5', x6', x7', x8', x9')
+                 (conj Hx0 (conj Hx1 (conj Hx2 (conj Hx3 (conj Hx4 (conj Hx5 (conj Hx6 (conj Hx7 (conj Hx8 Hx9)))))))))).
+  specialize (H1 (x0', x1', x2', x3', x4', x5', x6', x7', x8', x9')
+                 (conj Hx0 (conj Hx1 (conj Hx2 (conj Hx3 (conj Hx4 (conj Hx5 (conj Hx6 (conj Hx7 (conj Hx8 Hx9)))))))))).
+  Time let args := constr:(op10_args_to_bounded (x0', x1', x2', x3', x4', x5', x6', x7', x8', x9') Hx0 Hx1 Hx2 Hx3 Hx4 Hx5 Hx6 Hx7 Hx8 Hx9) in
+       admit; t_correct_and_bounded ropZ_sig Hbounds H0 H1 args. (* On 8.6beta1, with ~2 GB RAM, Finished transaction in 46.56 secs (46.372u,0.14s) (successful) *)
+Admitted. (*Time Qed. (* On 8.6beta1, with ~4.3 GB RAM, Finished transaction in 67.652 secs (66.932u,0.64s) (successful) *)*)
